Deep type checking
Bug fixes:

- Fix variable binding time (in `wp_decl_var`).
  Variables become available before they are initialized.
  This bug would have allowed us to verify a program like:
  ```
  int x = 0;
  { int x = x; }
  ```
  The second line should have UB because the `x` on the RHS refers
  to the declaration on line 2, not the one on line 1.

- Fix typing of globals `Eglobal`, adding `tref`

- Fix printer for decomposition decls (`Ddecompose`)

Also,

- Improve the shallow type checker
- Rework casts
- Improve members, member pointers, subscripts
- Hoist parsec, some traversals, and an error type

include/Formatter.hpp
@@ -34,6 +34,10 @@ public:
 	void indent();
 	void outdent();
 
+	void clear_spaces() {
+		spaces = 0;
+	}
+
 	void ascii(int c);
 
 	template<typename T>
