tests/cpp2v/test_member_pointer.t/test.cpp
@@ -6,10 +6,26 @@
 
 struct P {
     int x;
+    void foo();
+    virtual void bar();
 };
 
-int test() {
-    auto t = &P::x;
+void test() {
+    auto field = &P::x;
+    auto method = &P::foo;
+    auto vmethod = &P::bar;
+
     P x;
-    return x.*t;
+    P* p = &x;
+    static_cast<void>(x.*field);
+    static_cast<void>(p->*field);
+    x.foo();
+    p->foo();
+    (x.*method)();
+    (p->*method)();
+    x.bar();
+    p->bar();
+    (x.*vmethod)();
+    (p->*vmethod)();
+
 }
