theories/lang/cpp/logic/const.v
@@ -142,6 +142,7 @@ Section defs.
       | Tresult_member_call _ _ _
       | Tresult_member _ _
       | Tdecltype _
+      | Texprtype _
       | Tresult_parenlist _ _ => False
       end%I.
 
